Almost complete proof that homomorphisms are injective iff they have trivial kernel

src/Mitchell/group theory/group.lean
@@ -4,10 +4,12 @@
 -/
 
 import data.set.basic
+import init.function
 
 universes u v w
 variables {α : Type u} {β : Type v} {γ : Type w}
 
+-- Structure or class?
 structure is_homomorphism [group α] [group β] (f : α → β) : Prop :=
     (hom_mul : ∀ a b, f (a * b) = (f a) * (f b))
 
@@ -38,33 +40,84 @@ end
 end is_homomorphism
 
 
-class subgroup [group α] (s : set α) : Prop := 
+class is_subgroup [group α] (s : set α) : Prop := 
     (one_closed : (1 : α) ∈ s)
     (inv_closed : ∀ {a}, a ∈ s → a⁻¹ ∈ s) 
     (mul_closed : ∀ {a b}, a ∈ s → b ∈ s → a * b ∈ s) 
 
--- theorem int_subgroups (S : set ℤ) [group ℤ] [subgroup S] : ∃ a ∈ S, ∀ b ∈ S, a ∣ b := sorry
+attribute [simp] is_subgroup.one_closed is_subgroup.inv_closed is_subgroup.mul_closed
 
-namespace subgroup
+-- theorem int_subgroups (S : set ℤ) [group ℤ] [is_subgroup S] : ∃ a ∈ S, ∀ b ∈ S, a ∣ b := sorry
+
+namespace is_subgroup
 variables [group α] [group β]
-variables {s : set α}[subgroup s]
+variables {s : set α} [is_subgroup s]
 
-instance trivial : subgroup ({1} : set α) :=
+instance trivial : is_subgroup ({1} : set α) :=
     by refine {..}; by simp {contextual := tt}
 
-instance image {f : α → β} (hf: is_homomorphism f) : subgroup (f '' s) := {
-    subgroup .
-    mul_closed := assume c₁ c₂ ⟨b₁, hb₁, eq₁⟩ ⟨b₂, hb₂, eq₂⟩,
+instance image {f : α → β} (hf: is_homomorphism f) : is_subgroup (f '' s) := {
+    is_subgroup .
+    mul_closed := assume a₁ a₂ ⟨b₁, hb₁, eq₁⟩ ⟨b₂, hb₂, eq₂⟩,
     ⟨b₁ * b₂, mul_closed hb₁ hb₂, by simp [eq₁, eq₂, hf.hom_mul]⟩,
     one_closed := ⟨1, one_closed s, hf.one⟩,
     inv_closed := assume a ⟨b, hb, eq⟩,
     ⟨b⁻¹, inv_closed hb, by simp [eq, hf.inv]⟩ 
 }
 
-instance preimage {f : β → α} (hf : is_homomorphism f) : subgroup (f ⁻¹' s) :=
-    by refine {..}; simp [hf.hom_mul, hf.one, hf.inv, one_closed, inv_closed, mul_closed] {contextual:=tt}
+instance preimage {f : β → α} (hf : is_homomorphism f) : is_subgroup (f ⁻¹' s) :=
+    by refine {..}; simp [hf.hom_mul, hf.one, hf.inv] {contextual:=tt}
 
-instance kernel {f : α → β} (hf: is_homomorphism f) : subgroup (f ⁻¹' ({1} : set β)) := 
-    preimage hf
+def kernel {f : α → β} (hf: is_homomorphism f) : set α := {a | f a = 1}
 
-end subgroup
+instance kernel_subg {f : α → β} (hf: is_homomorphism f) : is_subgroup (kernel hf) := 
+    by refine {..}; simp [kernel, hf.hom_mul, hf.one, hf.inv] {contextual:=tt}
+
+def left_coset  (a : α) {s : set α} [is_subgroup s] : set α := {b | ∃ (g : s), b = a * g}
+def right_coset {s : set α} [is_subgroup s] (a : α) : set α := {b | ∃ (g : s), b = g * a}
+
+lemma kernel_iff_equiv {f : α → β} (hf: is_homomorphism f) (a b : α) : f b = f a ↔ a⁻¹ * b ∈ kernel hf :=
+begin
+    split,
+    {
+        assume h,
+        simp [kernel, has_mem.mem, set.mem, set_of], -- Is there a tactic which does this?
+        simp [hf.hom_mul, hf.inv, h]
+    },
+    {
+        assume h,
+        simp [kernel, has_mem.mem, set.mem, set_of] at h,
+        calc
+            f b = f (a * a⁻¹ * b)   : by simp; rw [mul_assoc]; simp [hf.hom_mul, h]
+            ... = f a               : by rw [mul_assoc]; simp [hf.hom_mul, h]
+    }
+    -- struggling with simp [mul_assoc]
+end
+
+theorem inj_iff_trivial_kernel {f : α → β} (hf: is_homomorphism f) : 
+    function.injective f ↔ kernel hf = {1} :=
+begin
+    split,
+    {
+        unfold function.injective,
+        assume h,
+        have hx : ∃ x, x ∈ kernel hf := ⟨1, hf.one⟩,
+        dsimp [kernel],
+        suffices ht : ∀ a, f a = 1 → a = 1, -- Doesn't work!
+        tactic.swap, -- Not necessary once suffices is working
+        assume a ha,
+        have hi : f a = f 1 := by simp [hf.one, ha],
+        simp [h hi, hf.one],
+        admit
+    },
+    {
+        assume h a b,
+        simp [kernel_iff_equiv hf b a, kernel, h],
+        assume hbia,
+        calc
+            a   = b * b⁻¹ * a     : by simp 
+            ... = b               : by rw mul_assoc; simp [hbia]
+    }
+end
+
+end is_subgroup
